Make everything dependent

Hashmap/AssocList/Basic.lean
@@ -6,7 +6,11 @@ Authors: Leonardo de Moura, Mario Carneiro, Markus Himmel
 import Hashmap.ForUpstream
 import Hashmap.BEq
 
+universe v u
+
 namespace Lean
+
+variable {α : Type u} {β : α → Type v}
 
 /--
 `AssocList α β` is "the same as" `List (α × β)`, but flattening the structure
@@ -14,12 +18,14 @@ leads to one fewer pointer indirection (in the current code generator).
 It is mainly intended as a component of `HashMap`, but it can also be used as a plain
 key-value map.
 -/
-inductive AssocList (α : Type u) (β : Type v) where
+inductive AssocList (α : Type u) (β : α → Type v) where
   /-- An empty list -/
   | nil
   /-- Add a `key, value` pair to the list -/
-  | cons (key : α) (value : β) (tail : AssocList α β)
+  | cons (key : α) (value : β key) (tail : AssocList α β)
   deriving Inhabited
+
+abbrev AssocList' (α : Type u) (β : Type v) := AssocList α (fun _ => β)
 
 namespace AssocList
 
@@ -28,27 +34,27 @@ namespace AssocList
 This is used to give specifications for all the `AssocList` functions
 in terms of corresponding list functions.
 -/
-def toList : AssocList α β → List (α × β)
+def toList : AssocList α β → List (Σ a, β a)
   | nil => []
-  | cons a b es => (a, b) :: es.toList
+  | cons a b es => ⟨a, b⟩ :: es.toList
 
 @[simp] theorem toList_nil : (nil : AssocList α β).toList = [] := rfl
-@[simp] theorem toList_cons {l : AssocList α β} {a : α} {b : β} : (l.cons a b).toList = (a, b) :: l.toList := rfl
+@[simp] theorem toList_cons {l : AssocList α β} {a : α} {b : β a} : (l.cons a b).toList = ⟨a, b⟩ :: l.toList := rfl
 
 /-- `O(n)`. Returns the first entry in the list whose key is equal to `a`. -/
-def findEntry? [BEq α] (a : α) : AssocList α β → Option (α × β)
+def findEntry? [BEq α] (a : α) : AssocList α β → Option (Σ a, β a)
   | nil => none
-  | cons k v es => bif k == a then some (k, v) else findEntry? a es
+  | cons k v es => bif k == a then some ⟨k, v⟩ else findEntry? a es
 
 @[simp] theorem findEntry?_nil [BEq α] {a : α} : (nil : AssocList α β).findEntry? a = none := rfl
-theorem findEntry?_cons [BEq α] {l : AssocList α β} {k a : α} {v : β} :
-    (l.cons k v).findEntry? a = bif k == a then some (k, v) else l.findEntry? a := rfl
+theorem findEntry?_cons [BEq α] {l : AssocList α β} {k a : α} {v : β k} :
+    (l.cons k v).findEntry? a = bif k == a then some ⟨k, v⟩ else l.findEntry? a := rfl
 
-theorem findEntry?_cons_of_true [BEq α] {l : AssocList α β} {k a : α} {v : β} (h : k == a) :
-    (l.cons k v).findEntry? a = some (k, v) := by
+theorem findEntry?_cons_of_true [BEq α] {l : AssocList α β} {k a : α} {v : β k} (h : k == a) :
+    (l.cons k v).findEntry? a = some ⟨k, v⟩ := by
   simp [findEntry?, h]
 
-theorem findEntry?_cons_of_false [BEq α] {l : AssocList α β} {k a : α} {v : β} (h : (k == a) = false) :
+theorem findEntry?_cons_of_false [BEq α] {l : AssocList α β} {k a : α} {v : β k} (h : (k == a) = false) :
     (l.cons k v).findEntry? a = l.findEntry? a := by
   simp [findEntry?, h]
 
@@ -62,23 +68,27 @@ theorem findEntry?_eq_of_beq [BEq α] [EquivBEq α] {l : AssocList α β} {a a' 
       rw [findEntry?_cons_of_false h', findEntry?_cons_of_false h₂, ih]
     · rw [findEntry?_cons_of_true h', findEntry?_cons_of_true (BEq.trans h' h)]
 
-def find? [BEq α] (a : α) : AssocList α β → Option β
+section
+
+variable {β : Type v}
+
+def find? [BEq α] (a : α) : AssocList' α β → Option β
   | nil => none
   | cons k v es => bif k == a then some v else find? a es
 
-@[simp] theorem find?_nil [BEq α] {a : α} : (nil : AssocList α β).find? a = none := rfl
-theorem find?_cons [BEq α] {l : AssocList α β} {k a : α} {v : β} :
+@[simp] theorem find?_nil [BEq α] {a : α} : (nil : AssocList' α β).find? a = none := rfl
+theorem find?_cons [BEq α] {l : AssocList' α β} {k a : α} {v : β} :
     (l.cons k v).find? a = bif k == a then some v else l.find? a := rfl
 
-theorem find?_cons_of_true [BEq α] {l : AssocList α β} {k a : α} {v : β} (h : k == a) :
+theorem find?_cons_of_true [BEq α] {l : AssocList' α β} {k a : α} {v : β} (h : k == a) :
     (l.cons k v).find? a = some v := by
   simp [find?, h]
 
-theorem find?_cons_of_false [BEq α] {l : AssocList α β} {k a : α} {v : β} (h : (k == a) = false) :
+theorem find?_cons_of_false [BEq α] {l : AssocList' α β} {k a : α} {v : β} (h : (k == a) = false) :
     (l.cons k v).find? a = l.find? a := by
   simp [find?, h]
 
-theorem find?_eq_findEntry? [BEq α] {l : AssocList α β} {a : α} :
+theorem find?_eq_findEntry? [BEq α] {l : AssocList' α β} {a : α} :
     l.find? a = (l.findEntry? a).map (·.2) := by
   induction l
   · simp
@@ -87,23 +97,25 @@ theorem find?_eq_findEntry? [BEq α] {l : AssocList α β} {a : α} :
     · rw [findEntry?_cons_of_false h, find?_cons_of_false h, ih]
     · rw [findEntry?_cons_of_true h, find?_cons_of_true h, Option.map_some']
 
-theorem find?_eq_of_beq [BEq α] [EquivBEq α] {l : AssocList α β} {a a' : α} (h : a == a') :
+theorem find?_eq_of_beq [BEq α] [EquivBEq α] {l : AssocList' α β} {a a' : α} (h : a == a') :
     l.find? a = l.find? a' := by
   simp [find?_eq_findEntry?, findEntry?_eq_of_beq h]
+
+end
 
 def findKey? [BEq α] (a : α) : AssocList α β → Option α
   | nil => none
   | cons k _ es => bif k == a then some k else findKey? a es
 
 @[simp] theorem findKey?_nil [BEq α] {a : α} : (nil : AssocList α β).findKey? a = none := rfl
-theorem findKey?_cons [BEq α] {l : AssocList α β} {k a : α} {v : β} :
+theorem findKey?_cons [BEq α] {l : AssocList α β} {k a : α} {v : β k} :
     (l.cons k v).findKey? a = bif k == a then some k else l.findKey? a := rfl
 
-theorem findKey?_cons_of_true [BEq α] {l : AssocList α β} {k a : α} {v : β} (h : k == a) :
+theorem findKey?_cons_of_true [BEq α] {l : AssocList α β} {k a : α} {v : β k} (h : k == a) :
     (l.cons k v).findKey? a = some k := by
   simp [findKey?, h]
 
-theorem findKey?_cons_of_false [BEq α] {l : AssocList α β} {k a : α} {v : β} (h : (k == a) = false) :
+theorem findKey?_cons_of_false [BEq α] {l : AssocList α β} {k a : α} {v : β k} (h : (k == a) = false) :
     (l.cons k v).findKey? a = l.findKey? a := by
   simp [findKey?, h]
 
@@ -125,29 +137,29 @@ def contains [BEq α] (a : α) : AssocList α β → Bool
   | cons k _ l => k == a || l.contains a
 
 @[simp] theorem contains_nil [BEq α] {a : α} : (nil : AssocList α β).contains a = false := rfl
-@[simp] theorem contains_cons [BEq α] {l : AssocList α β} {k a : α} {v : β} :
+@[simp] theorem contains_cons [BEq α] {l : AssocList α β} {k a : α} {v : β k} :
     (l.cons k v).contains a = (k == a || l.contains a) := rfl
 
-theorem contains_cons_eq_false [BEq α] {l : AssocList α β} {k a : α} {v : β} :
+theorem contains_cons_eq_false [BEq α] {l : AssocList α β} {k a : α} {v : β k} :
     ((l.cons k v).contains a = false) ↔ ((k == a) = false) ∧ (l.contains a = false) := by
   rw [Bool.eq_iff_iff]
   simp [contains_cons, not_or]
 
-theorem contains_cons_eq_true [BEq α] {l : AssocList α β} {k a : α} {v : β} :
+theorem contains_cons_eq_true [BEq α] {l : AssocList α β} {k a : α} {v : β k} :
     ((l.cons k v).contains a) ↔ (k == a) ∨ (l.contains a) := by
   rw [Bool.eq_iff_iff]
   simp [contains_cons]
 
-theorem contains_cons_of_beq [BEq α] {l : AssocList α β} {k a : α} {v : β} (h : k == a) :
+theorem contains_cons_of_beq [BEq α] {l : AssocList α β} {k a : α} {v : β k} (h : k == a) :
     (l.cons k v).contains a := contains_cons_eq_true.2 <| Or.inl h
 
-theorem contains_cons_self [BEq α] [EquivBEq α] {l : AssocList α β} {k : α} {v : β} :
+theorem contains_cons_self [BEq α] [EquivBEq α] {l : AssocList α β} {k : α} {v : β k} :
     (l.cons k v).contains k := contains_cons_of_beq BEq.refl
 
-theorem contains_cons_of_contains [BEq α] {l : AssocList α β} {k a : α} {v : β} (h : l.contains a) :
+theorem contains_cons_of_contains [BEq α] {l : AssocList α β} {k a : α} {v : β k} (h : l.contains a) :
     (l.cons k v).contains a := contains_cons_eq_true.2 <| Or.inr h
 
-theorem contains_of_contains_cons [BEq α] {l : AssocList α β} {k a : α} {v : β} (h₁ : (l.cons k v).contains a)
+theorem contains_of_contains_cons [BEq α] {l : AssocList α β} {k a : α} {v : β k} (h₁ : (l.cons k v).contains a)
     (h₂ : (k == a) = false) : l.contains a := by
   rcases (contains_cons_eq_true.1 h₁) with (h|h)
   · exact False.elim (Bool.eq_false_iff.1 h₂ h)
@@ -162,7 +174,7 @@ theorem contains_eq_isSome_findEntry? [BEq α] {l : AssocList α β} {a : α} :
     · simp [findEntry?_cons_of_false h, h, ih]
     · simp [findEntry?_cons_of_true h, h]
 
-theorem contains_eq_isSome_find? [BEq α] {l : AssocList α β} {a : α} :
+theorem contains_eq_isSome_find? {β : Type v} [BEq α] {l : AssocList' α β} {a : α} :
     l.contains a = (l.find? a).isSome := by
   simp [contains_eq_isSome_findEntry?, find?_eq_findEntry?]
 
@@ -178,23 +190,23 @@ theorem contains_of_beq [BEq α] [EquivBEq α] {l : AssocList α β} {a b : α} 
     l.contains b := by
   rwa [← contains_eq_of_beq hab]
 
-def findEntry [BEq α] (l : AssocList α β) (a : α) (h : l.contains a) : α × β :=
+def findEntry [BEq α] (l : AssocList α β) (a : α) (h : l.contains a) : Σ a, β a :=
   (l.findEntry? a).get <| contains_eq_isSome_findEntry?.symm.trans h
 
 theorem findEntry?_eq_some_findEntry [BEq α] {l : AssocList α β} {a : α} (h : l.contains a) :
     l.findEntry? a = some (l.findEntry a h) := by
   simp [findEntry]
 
-theorem findEntry_cons_of_beq [BEq α] {l : AssocList α β} {k a : α} {v : β} (h : k == a) :
-    (l.cons k v).findEntry a (contains_cons_of_beq h) = (k, v) := by
+theorem findEntry_cons_of_beq [BEq α] {l : AssocList α β} {k a : α} {v : β k} (h : k == a) :
+    (l.cons k v).findEntry a (contains_cons_of_beq h) = ⟨k, v⟩ := by
   simp [findEntry, findEntry?_cons_of_true h]
 
 @[simp]
-theorem findEntry_cons_self [BEq α] [EquivBEq α] {l : AssocList α β} {k : α} {v : β} :
-    (l.cons k v).findEntry k contains_cons_self = (k, v) :=
+theorem findEntry_cons_self [BEq α] [EquivBEq α] {l : AssocList α β} {k : α} {v : β k} :
+    (l.cons k v).findEntry k contains_cons_self = ⟨k, v⟩ :=
   findEntry_cons_of_beq BEq.refl
 
-theorem findEntry_cons_of_false [BEq α] {l : AssocList α β} {k a : α} {v : β} {h₁ : (l.cons k v).contains a}
+theorem findEntry_cons_of_false [BEq α] {l : AssocList α β} {k a : α} {v : β k} {h₁ : (l.cons k v).contains a}
     (h₂ : (k == a) = false) : (l.cons k v).findEntry a h₁ = l.findEntry a (contains_of_contains_cons h₁ h₂) := by
   simp [findEntry, findEntry?_cons_of_false h₂]
 
@@ -205,16 +217,16 @@ theorem findKey?_eq_some_findKey [BEq α] {l : AssocList α β} {a : α} (h : l.
     l.findKey? a = some (l.findKey a h) := by
   simp [findKey]
 
-theorem findKey_cons_of_beq [BEq α] {l : AssocList α β} {k a : α} {v : β} (h : k == a) :
+theorem findKey_cons_of_beq [BEq α] {l : AssocList α β} {k a : α} {v : β k} (h : k == a) :
     (l.cons k v).findKey a (contains_cons_of_beq h) = k := by
   simp [findKey, findKey?_cons_of_true h]
 
 @[simp]
-theorem findKey_cons_self [BEq α] [EquivBEq α] {l : AssocList α β} {k : α} {v : β} :
+theorem findKey_cons_self [BEq α] [EquivBEq α] {l : AssocList α β} {k : α} {v : β k} :
     (l.cons k v).findKey k contains_cons_self = k :=
   findKey_cons_of_beq BEq.refl
 
-theorem findKey_cons_of_false [BEq α] {l : AssocList α β} {k a : α} {v : β} {h₁ : (l.cons k v).contains a}
+theorem findKey_cons_of_false [BEq α] {l : AssocList α β} {k a : α} {v : β k} {h₁ : (l.cons k v).contains a}
     (h₂ : (k == a) = false) : (l.cons k v).findKey a h₁ = l.findKey a (contains_of_contains_cons h₁ h₂) := by
   simp [findKey, findKey?_cons_of_false h₂]
 
@@ -227,43 +239,49 @@ theorem findKey_beq [BEq α] {l : AssocList α β} {a : α} {h : l.contains a} :
       exact @ih (contains_of_contains_cons h h')
     · rwa [findKey_cons_of_beq h']
 
-def find [BEq α] (l : AssocList α β) (a : α) (h : l.contains a) : β :=
+section
+
+variable {β : Type v}
+
+def find [BEq α] (l : AssocList' α β) (a : α) (h : l.contains a) : β :=
   (l.find? a).get <| contains_eq_isSome_find?.symm.trans h
 
-theorem find?_eq_some_find [BEq α] {l : AssocList α β} {a : α} (h : l.contains a) :
+theorem find?_eq_some_find [BEq α] {l : AssocList' α β} {a : α} (h : l.contains a) :
     l.find? a = some (l.find a h) := by
   simp [find]
 
-theorem find_cons_of_beq [BEq α] {l : AssocList α β} {k a : α} {v : β} (h : k == a) :
+theorem find_cons_of_beq [BEq α] {l : AssocList' α β} {k a : α} {v : β} (h : k == a) :
     (l.cons k v).find a (contains_cons_of_beq h) = v := by
   simp [find, find?_cons_of_true h]
 
 @[simp]
-theorem find_cons_self [BEq α] [EquivBEq α] {l : AssocList α β} {k : α} {v : β} :
+theorem find_cons_self [BEq α] [EquivBEq α] {l : AssocList' α β} {k : α} {v : β} :
     (l.cons k v).find k contains_cons_self = v :=
   find_cons_of_beq BEq.refl
 
-theorem find_cons_of_false [BEq α] {l : AssocList α β} {k a : α} {v : β} {h₁ : (l.cons k v).contains a}
+theorem find_cons_of_false [BEq α] {l : AssocList' α β} {k a : α} {v : β} {h₁ : (l.cons k v).contains a}
     (h₂ : (k == a) = false) : (l.cons k v).find a h₁ = l.find a (contains_of_contains_cons h₁ h₂) := by
   simp [find, find?_cons_of_false h₂]
 
-def replace [BEq α] (a : α) (b : β) : AssocList α β → AssocList α β
+end
+
+def replace [BEq α] (a : α) (b : β a) : AssocList α β → AssocList α β
   | nil => nil
-  | cons k v l => bif k == a then cons k b l else cons k v (replace a b l)
+  | cons k v l => bif k == a then cons a b l else cons k v (replace a b l)
 
-@[simp] theorem replace_nil [BEq α] {a : α} {b : β} : nil.replace a b = nil := rfl
-theorem replace_cons [BEq α] {l : AssocList α β} {k a : α} {v b : β} :
-    (l.cons k v).replace a b = bif k == a then l.cons k b else (l.replace a b).cons k v := rfl
+@[simp] theorem replace_nil [BEq α] {a : α} {b : β a} : nil.replace a b = nil := rfl
+theorem replace_cons [BEq α] {l : AssocList α β} {k a : α} {v : β k} {b : β a} :
+    (l.cons k v).replace a b = bif k == a then l.cons a b else (l.replace a b).cons k v := rfl
 
-theorem replace_cons_of_true [BEq α] {l : AssocList α β} {k a : α} {v b : β} (h : k == a) :
-    (l.cons k v).replace a b = l.cons k b := by
+theorem replace_cons_of_true [BEq α] {l : AssocList α β} {k a : α} {v : β k} {b : β a} (h : k == a) :
+    (l.cons k v).replace a b = l.cons a b := by
   simp [replace, h]
 
-theorem replace_cons_of_false [BEq α] {l : AssocList α β} {k a : α} {v b : β} (h : (k == a) = false) :
+theorem replace_cons_of_false [BEq α] {l : AssocList α β} {k a : α} {v : β k} {b : β a} (h : (k == a) = false) :
     (l.cons k v).replace a b = (l.replace a b).cons k v := by
   simp [replace, h]
 
-theorem replace_of_contains_eq_false [BEq α] {l : AssocList α β} {a : α} {b : β} (h : l.contains a = false) :
+theorem replace_of_contains_eq_false [BEq α] {l : AssocList α β} {a : α} {b : β a} (h : l.contains a = false) :
     l.replace a b = l := by
   induction l
   · simp
@@ -271,11 +289,11 @@ theorem replace_of_contains_eq_false [BEq α] {l : AssocList α β} {a : α} {b 
     rw [contains_cons_eq_false] at h
     rw [replace_cons_of_false h.1, ih h.2]
 
-theorem findEntry?_replace_of_contains_eq_false [BEq α] {l : AssocList α β} {k a : α} {b : β}
+theorem findEntry?_replace_of_contains_eq_false [BEq α] {l : AssocList α β} {k a : α} {b : β a}
     (hl : l.contains a = false) : (l.replace a b).findEntry? k = l.findEntry? k := by
   rw [replace_of_contains_eq_false hl]
 
-theorem findEntry?_replace_of_false [BEq α] [EquivBEq α] {l : AssocList α β} {k a : α} {b : β}
+theorem findEntry?_replace_of_false [BEq α] [EquivBEq α] {l : AssocList α β} {k a : α} {b : β a}
     (h : (k == a) = false) : (l.replace a b).findEntry? k = l.findEntry? k := by
   induction l
   · simp
@@ -284,10 +302,10 @@ theorem findEntry?_replace_of_false [BEq α] [EquivBEq α] {l : AssocList α β}
     · rw [replace_cons_of_false h', findEntry?_cons, findEntry?_cons, ih]
     · rw [replace_cons_of_true h']
       have hk : (k' == k) = false := BEq.neq_of_beq_of_neq h' (BEq.symm_false h)
-      simp [findEntry?_cons_of_false hk]
+      simp [findEntry?_cons_of_false (BEq.symm_false h), findEntry?_cons_of_false hk]
 
-theorem findEntry?_replace_of_true [BEq α] [EquivBEq α] {l : AssocList α β} {k a : α} {b : β} (hl : l.contains a = true)
-    (h : k == a) : (l.replace a b).findEntry? k = some (l.findKey k (contains_of_beq hl (BEq.symm h)), b) := by
+theorem findEntry?_replace_of_true [BEq α] [EquivBEq α] {l : AssocList α β} {k a : α} {b : β a} (hl : l.contains a = true)
+    (h : k == a) : (l.replace a b).findEntry? k = some ⟨a, b⟩ := by
   induction l
   · simp at hl
   · next k' v' l ih =>
@@ -295,74 +313,74 @@ theorem findEntry?_replace_of_true [BEq α] [EquivBEq α] {l : AssocList α β} 
     · rw [replace_cons_of_false hk'a]
       have hk'k : (k' == k) = false := BEq.neq_of_neq_of_beq hk'a (BEq.symm h)
       rw [findEntry?_cons_of_false hk'k]
-      have hl'₂ : l.contains a = true := contains_of_contains_cons hl hk'a
-      rw [findKey_cons_of_false hk'k, ih hl'₂]
-    · rw [replace_cons_of_true hk'a]
-      have hkk' : k' == k := by
-        exact BEq.trans hk'a (BEq.symm h)
-      rw [findEntry?_cons_of_true hkk', findKey_cons_of_beq hkk']
+      exact ih (contains_of_contains_cons hl hk'a)
+    · rw [replace_cons_of_true hk'a, findEntry?_cons_of_true (BEq.symm h)]
 
-theorem find?_replace_of_contains_eq_false [BEq α] {l : AssocList α β} {k a : α} {b : β}
+section
+
+variable {β : Type v}
+
+theorem find?_replace_of_contains_eq_false [BEq α] {l : AssocList' α β} {k a : α} {b : β}
     (hl : l.contains a = false) : (l.replace a b).find? k = l.find? k := by
   simp [find?_eq_findEntry?, findEntry?_replace_of_contains_eq_false hl]
 
-theorem find?_replace_of_false [BEq α] [EquivBEq α] {l : AssocList α β} {k a : α} {b : β}
+theorem find?_replace_of_false [BEq α] [EquivBEq α] {l : AssocList' α β} {k a : α} {b : β}
     (h : (k == a) = false) : (l.replace a b).find? k = l.find? k := by
   simp [find?_eq_findEntry?, findEntry?_replace_of_false h]
 
-theorem find?_replace_of_true [BEq α] [EquivBEq α] {l : AssocList α β} {k a : α} {b : β}
+theorem find?_replace_of_true [BEq α] [EquivBEq α] {l : AssocList' α β} {k a : α} {b : β}
     (hl : l.contains a = true) (h : k == a) : (l.replace a b).find? k = some b := by
   simp [find?_eq_findEntry?, findEntry?_replace_of_true hl h]
 
-theorem findKey?_replace_of_contains_eq_false [BEq α] {l : AssocList α β} {k a : α} {b : β}
+end
+
+theorem findKey?_replace_of_contains_eq_false [BEq α] {l : AssocList α β} {k a : α} {b : β a}
     (hl : l.contains a = false) : (l.replace a b).findKey? k = l.findKey? k := by
   simp [findKey?_eq_findEntry?, findEntry?_replace_of_contains_eq_false hl]
 
-theorem findKey?_replace_of_false [BEq α] [EquivBEq α] {l : AssocList α β} {k a : α} {b : β}
+theorem findKey?_replace_of_false [BEq α] [EquivBEq α] {l : AssocList α β} {k a : α} {b : β a}
     (h : (k == a) = false) : (l.replace a b).findKey? k = l.findKey? k := by
   simp [findKey?_eq_findEntry?, findEntry?_replace_of_false h]
 
-theorem findKey?_replace_of_true [BEq α] [EquivBEq α] {l : AssocList α β} {k a : α} {b : β}
-    (hl : l.contains a = true) (h : (k == a)) :
-    (l.replace a b).findKey? k = some (l.findKey k (contains_of_beq hl (BEq.symm h))) := by
+theorem findKey?_replace_of_true [BEq α] [EquivBEq α] {l : AssocList α β} {k a : α} {b : β a}
+    (hl : l.contains a = true) (h : (k == a)) : (l.replace a b).findKey? k = some a := by
   simp [findKey?_eq_findEntry?, findEntry?_replace_of_true hl h]
 
-theorem findKey?_replace_of_true' [BEq α] [EquivBEq α] {l : AssocList α β} {k a : α} {b : β}
-    (hl : l.contains a = true) (h : (k == a)) : (l.replace a b).findKey? k = l.findKey? k := by
-  rw [findKey?_replace_of_true hl h, findKey?_eq_some_findKey]
-
-@[simp]
-theorem findKey?_replace [BEq α] [EquivBEq α] {l : AssocList α β} {k a : α} {b : β} :
-    (l.replace a b).findKey? k = l.findKey? k := by
+theorem findKey?_replace [BEq α] [EquivBEq α] {l : AssocList α β} {k a : α} {b : β a} :
+    (l.replace a b).findKey? k = bif l.contains a && k == a then some a else l.findKey? k := by
   cases hl : l.contains a
-  · rw [findKey?_replace_of_contains_eq_false hl]
+  · simp [findKey?_replace_of_contains_eq_false hl]
   · cases h : k == a
-    · rw [findKey?_replace_of_false h]
-    · rw [findKey?_replace_of_true' hl h]
+    · simp [findKey?_replace_of_false h]
+    · simp [findKey?_replace_of_true hl h]
 
 @[simp]
-theorem contains_replace [BEq α] [EquivBEq α] {l : AssocList α β} {k a : α} {b : β} :
-    (l.replace k v).contains a = l.contains a := by
-  simp [contains_eq_isSome_findKey?]
+theorem contains_replace [BEq α] [EquivBEq α] {l : AssocList α β} {k a : α} {b : β a} :
+    (l.replace a b).contains k = l.contains k := by
+  cases h : l.contains a && k == a
+  · rw [contains_eq_isSome_findKey?, findKey?_replace, h, cond_false, contains_eq_isSome_findKey?]
+  · rw [contains_eq_isSome_findKey?, findKey?_replace, h, cond_true, Option.isSome_some, Eq.comm]
+    rw [Bool.and_eq_true] at h
+    exact contains_of_beq h.1 (BEq.symm h.2)
 
 def erase [BEq α] (a : α) : AssocList α β → AssocList α β
   | nil => nil
   | cons k v l => bif k == a then l else cons k v (l.erase a)
 
 @[simp] theorem erase_nil [BEq α] {a : α} : (nil : AssocList α β).erase a = nil := rfl
-theorem erase_cons [BEq α] {l : AssocList α β} {k a : α} {v : β} :
+theorem erase_cons [BEq α] {l : AssocList α β} {k a : α} {v : β k} :
     (l.cons k v).erase a = bif k == a then l else cons k v (l.erase a) := rfl
 
-theorem erase_cons_of_beq [BEq α] {l : AssocList α β} {k a : α} {v : β} (h : k == a) :
+theorem erase_cons_of_beq [BEq α] {l : AssocList α β} {k a : α} {v : β k} (h : k == a) :
     (l.cons k v).erase a = l :=
   by simp [erase_cons, h]
 
 @[simp]
-theorem erase_cons_self [BEq α] [EquivBEq α] {l : AssocList α β} {k : α} {v : β} :
+theorem erase_cons_self [BEq α] [EquivBEq α] {l : AssocList α β} {k : α} {v : β k} :
     (l.cons k v).erase k = l :=
   erase_cons_of_beq BEq.refl
 
-theorem erase_cons_of_false [BEq α] {l : AssocList α β} {k a : α} {v : β} (h : (k == a) = false) :
+theorem erase_cons_of_false [BEq α] {l : AssocList α β} {k a : α} {v : β k} (h : (k == a) = false) :
     (l.cons k v).erase a = (l.erase a).cons k v := by
   simp [erase_cons, h]
 
@@ -376,14 +394,14 @@ def keys : AssocList α β → List α
   | cons k _ l => k :: (keys l)
 
 @[simp] theorem keys_nil : (nil : AssocList α β).keys = [] := rfl
-@[simp] theorem keys_cons {l : AssocList α β} {k : α} {v : β} : (l.cons k v).keys = k :: l.keys := rfl
+@[simp] theorem keys_cons {l : AssocList α β} {k : α} {v : β k} : (l.cons k v).keys = k :: l.keys := rfl
 
-@[simp]
-theorem keys_replace [BEq α] {l : AssocList α β} {a : α} {b : β} : (l.replace a b).keys = l.keys := by
-  induction l
-  · simp
-  · next k v t ih =>
-    simp [replace_cons, apply_bif keys, ih]
+-- @[simp]
+-- theorem keys_replace [BEq α] {l : AssocList α β} {a : α} {b : β a} : (l.replace a b).keys = l.keys := by
+--   induction l
+--   · simp
+--   · next k v t ih =>
+--     simp [replace_cons, apply_bif keys, ih]
 
 theorem contains_eq_keys_contains [BEq α] [EquivBEq α] {l : AssocList α β} {a : α} :
     l.contains a = l.keys.contains a := by
@@ -417,7 +435,7 @@ theorem contains_eq_false_iff_forall [BEq α] [EquivBEq α] {l : AssocList α β
   simp only [Bool.eq_false_iff, ne_eq, contains_iff_exists, not_exists, not_and]
 
 @[simp]
-theorem WF_cons_iff [BEq α] [EquivBEq α] {l : AssocList α β} {k : α} {v : β} :
+theorem WF_cons_iff [BEq α] [EquivBEq α] {l : AssocList α β} {k : α} {v : β k} :
     (l.cons k v).WF ↔ l.WF ∧ (l.contains k) = false := by
   refine ⟨fun ⟨h⟩ => ?_, fun ⟨⟨h₁⟩, h₂⟩ => ⟨?_⟩⟩
   · rw [keys_cons, List.pairwise_cons] at h
@@ -425,61 +443,78 @@ theorem WF_cons_iff [BEq α] [EquivBEq α] {l : AssocList α β} {k : α} {v : �
   · rw [keys_cons, List.pairwise_cons, ← contains_eq_false_iff_forall]
     exact ⟨h₂, h₁⟩
 
-theorem WF_replace [BEq α] [EquivBEq α] {l : AssocList α β} {k : α} {v : β} : l.WF → (l.replace k v).WF :=
-  WF_of_keys_eq keys_replace.symm
+theorem WF_replace [BEq α] [EquivBEq α] {l : AssocList α β} {k : α} {v : β k} (h : l.WF) : (l.replace k v).WF := by
+  induction l
+  · simp
+  · next k' v' l ih =>
+    rw [WF_cons_iff] at h
+    cases hk'k : k' == k
+    · rw [replace_cons_of_false hk'k, WF_cons_iff]
+      refine ⟨ih h.1, ?_⟩
+      simpa using h.2
+    · rw [replace_cons_of_true hk'k, WF_cons_iff]
+      refine ⟨h.1, ?_⟩
+      simpa [contains_eq_of_beq (BEq.symm hk'k)] using h.2
 
-def insert [BEq α] (l : AssocList α β) (k : α) (v : β) : AssocList α β :=
+def insert [BEq α] (l : AssocList α β) (k : α) (v : β k) : AssocList α β :=
   bif l.contains k then l.replace k v else l.cons k v
 
-theorem insert_of_contains [BEq α] {l : AssocList α β} {k : α} {v : β} (h : l.contains k) :
+theorem insert_of_contains [BEq α] {l : AssocList α β} {k : α} {v : β k} (h : l.contains k) :
     l.insert k v = l.replace k v := by
   simp [insert, h]
 
-theorem insert_of_contains_eq_false [BEq α] {l : AssocList α β} {k : α} {v : β} (h : l.contains k = false) :
+theorem insert_of_contains_eq_false [BEq α] {l : AssocList α β} {k : α} {v : β k} (h : l.contains k = false) :
     l.insert k v = l.cons k v := by
   simp [insert, h]
 
-theorem WF_insert [BEq α] [EquivBEq α] {l : AssocList α β} {k : α} {v : β} (h : l.WF) : (l.insert k v).WF := by
+theorem WF_insert [BEq α] [EquivBEq α] {l : AssocList α β} {k : α} {v : β k} (h : l.WF) : (l.insert k v).WF := by
   cases h' : l.contains k
   · rw [insert_of_contains_eq_false h', WF_cons_iff]
     exact ⟨h, h'⟩
   · rw [insert_of_contains h']
     exact WF_replace h
 
-theorem find?_insert_of_beq [BEq α] [EquivBEq α] {l : AssocList α β} {k a : α} {v : β} (h : k == a) :
+section
+
+variable {β : Type v}
+
+theorem find?_insert_of_beq [BEq α] [EquivBEq α] {l : AssocList' α β} {k a : α} {v : β} (h : k == a) :
     (l.insert k v).find? a = some v := by
   cases h' : l.contains k
   · rw [insert_of_contains_eq_false h', find?_cons_of_true h]
   · rw [insert_of_contains h', find?_replace_of_true h' (BEq.symm h)]
 
-theorem find?_insert_of_self [BEq α] [EquivBEq α] {l : AssocList α β} {k : α} {v : β} :
+theorem find?_insert_of_self [BEq α] [EquivBEq α] {l : AssocList' α β} {k : α} {v : β} :
     (l.insert k v).find? k = some v :=
   find?_insert_of_beq BEq.refl
 
-theorem find?_insert_of_false [BEq α] [EquivBEq α] {l : AssocList α β} {k a : α} {v : β} (h : (k == a) = false) :
+theorem find?_insert_of_false [BEq α] [EquivBEq α] {l : AssocList' α β} {k a : α} {v : β} (h : (k == a) = false) :
     (l.insert k v).find? a = l.find? a := by
   cases h' : l.contains k
   · rw [insert_of_contains_eq_false h', find?_cons_of_false h]
   · rw [insert_of_contains h', find?_replace_of_false (BEq.symm_false h)]
 
 -- TODO: would this be a reasonable simp lemma?
-theorem find?_insert [BEq α] [EquivBEq α] {l : AssocList α β} {k a : α} {v : β} :
+theorem find?_insert [BEq α] [EquivBEq α] {l : AssocList' α β} {k a : α} {v : β} :
     (l.insert k v).find? a = bif k == a then some v else l.find? a := by
   cases h : k == a
   · simp [find?_insert_of_false h, h]
   · simp [find?_insert_of_beq h, h]
 
-theorem findKey?_insert_of_contains [BEq α] [EquivBEq α] {l : AssocList α β} {k a : α} {v : β}
-    (h : l.contains k) : (l.insert k v).findKey? a = l.findKey? a := by
-  simp [insert_of_contains h]
+end
 
-theorem findKey?_insert_of_contains_eq_false [BEq α] [EquivBEq α] {l : AssocList α β} {k a : α} {v : β}
+-- TODO: Unify order in `bif k == a` vs. `bif a == k`.
+theorem findKey?_insert_of_contains [BEq α] [EquivBEq α] {l : AssocList α β} {k a : α} {v : β k}
+    (h : l.contains k) : (l.insert k v).findKey? a = bif k == a then some k else l.findKey? a := by
+  simp [insert_of_contains h, findKey?_replace, h, BEq.comm]
+
+theorem findKey?_insert_of_contains_eq_false [BEq α] [EquivBEq α] {l : AssocList α β} {k a : α} {v : β k}
     (hl : (l.contains k) = false) :
     (l.insert k v).findKey? a = bif k == a then some k else l.findKey? a := by
   simp [insert_of_contains_eq_false hl, findKey?_cons]
 
-theorem findKey?_insert [BEq α] [EquivBEq α] {l : AssocList α β} {k a : α} {v : β} :
-    (l.insert k v).findKey? a = bif !(l.contains k) && k == a then some k else l.findKey? a := by
+theorem findKey?_insert [BEq α] [EquivBEq α] {l : AssocList α β} {k a : α} {v : β k} :
+    (l.insert k v).findKey? a = bif k == a then some k else l.findKey? a := by
   cases hl : l.contains k
   · simp [findKey?_insert_of_contains_eq_false hl, hl]
   · simp [findKey?_insert_of_contains hl]
@@ -487,19 +522,19 @@ theorem findKey?_insert [BEq α] [EquivBEq α] {l : AssocList α β} {k a : α} 
 -- TODO: results about findEntry?+insert
 
 @[simp]
-theorem contains_insert [BEq α] [EquivBEq α] {l : AssocList α β} {k a : α} {v : β} :
+theorem contains_insert [BEq α] [EquivBEq α] {l : AssocList α β} {k a : α} {v : β k} :
     (l.insert k v).contains a = ((k == a) || l.contains a) := by
-  rw [contains_eq_isSome_find?, contains_eq_isSome_find?, find?_insert]
+  rw [contains_eq_isSome_findKey?, contains_eq_isSome_findKey?, findKey?_insert]
   cases k == a
   · simp
   · simp
 
-theorem contains_insert_of_beq [BEq α] [EquivBEq α] {l : AssocList α β} {k a : α} {v : β} (h : k == a) :
+theorem contains_insert_of_beq [BEq α] [EquivBEq α] {l : AssocList α β} {k a : α} {v : β k} (h : k == a) :
     (l.insert k v).contains a := by
   simp [h]
 
 @[simp]
-theorem contains_insert_self [BEq α] [EquivBEq α] {l : AssocList α β} {k : α} {v : β} :
+theorem contains_insert_self [BEq α] [EquivBEq α] {l : AssocList α β} {k : α} {v : β k} :
     (l.insert k v).contains k :=
   contains_insert_of_beq BEq.refl
 
@@ -553,21 +588,27 @@ theorem findEntry?_erase [BEq α] [EquivBEq α] {l : AssocList α β} {k a : α}
   · simp [findEntry?_erase_of_false h, h]
   · simp [findEntry?_erase_of_beq hl h, h]
 
-theorem find?_erase_self [BEq α] [EquivBEq α] {l : AssocList α β} {k : α} (h : l.WF) :
+section
+
+variable {β : Type v}
+
+theorem find?_erase_self [BEq α] [EquivBEq α] {l : AssocList' α β} {k : α} (h : l.WF) :
     (l.erase k).find? k = none := by
   simp [find?_eq_findEntry?, findEntry?_erase_self h]
 
-theorem find?_erase_of_beq [BEq α] [EquivBEq α] {l : AssocList α β} {k a : α} (hl : l.WF)
+theorem find?_erase_of_beq [BEq α] [EquivBEq α] {l : AssocList' α β} {k a : α} (hl : l.WF)
     (hka : k == a) : (l.erase k).find? a = none := by
   simp [find?_eq_findEntry?, findEntry?_erase_of_beq hl hka]
 
-theorem find?_erase_of_false [BEq α] [EquivBEq α] {l : AssocList α β} {k a : α}
+theorem find?_erase_of_false [BEq α] [EquivBEq α] {l : AssocList' α β} {k a : α}
     (hka : (k == a) = false) : (l.erase k).find? a = l.find? a := by
   simp [find?_eq_findEntry?, findEntry?_erase_of_false hka]
 
-theorem find?_erase [BEq α] [EquivBEq α] {l : AssocList α β} {k a : α} (hl : l.WF) :
+theorem find?_erase [BEq α] [EquivBEq α] {l : AssocList' α β} {k a : α} (hl : l.WF) :
     (l.erase k).find? a = bif k == a then none else l.find? a := by
   simp [find?_eq_findEntry?, findEntry?_erase hl, apply_bif (Option.map _)]
+
+end
 
 theorem findKey?_erase_self [BEq α] [EquivBEq α] {l : AssocList α β} {k : α} (h : l.WF) :
     (l.erase k).findKey? k = none := by
